











# FFT 的应用
一维的高斯分布为

$$
g(x) = \frac{1}{\sqrt{2\pi}\sigma}e^{-\frac{x^2}{2\sigma^2}}
$$

将两个一维高斯分布合并成一个二维高斯分布

$$
\begin{align*}
g(x,y) &= \frac{1}{\sqrt{2\pi}\sigma_x}\exp({-\frac{x^2}{2\sigma_x^2}}) \frac{1}{\sqrt{2\pi}\sigma_y}\exp({-\frac{y^2}{2\sigma_y^2}})\\
&= \frac{1}{2\pi\sigma_x\sigma_y}\exp({-\frac{x^2}{2\sigma_x^2}})\exp({-\frac{y^2}{2\sigma_y^2}})\\
&= \frac{1}{2\pi\sigma_x\sigma_y}\exp({-\frac{x^2}{2\sigma_x^2} - \frac{y^2}{2\sigma_y^2}})
\end{align*}
$$

在数值计算中我们对$-\frac{x^2}{2\sigma_x^2} - \frac{y^2}{2\sigma_y^2}$进行简化
$$
\begin{align*}
-\frac{x^2}{2\sigma_x^2} - \frac{y^2}{2\sigma_y^2}
&=-\frac{1}{2}\left(\frac{x^2}{\sigma_x^2} + \frac{y^2}{\sigma_y^2}\right)\\
&=-\frac{1}{2}\left(\frac{x^2\sigma_y^2 + y^2\sigma_x^2}{\sigma_x^2\sigma_y^2}\right)\\
&=-\frac{1}{2}\left(\frac{(x\sigma_y)^2 + (y\sigma_x)^2}{(\sigma_x\sigma_y)^2}\right)\\
\end{align*}
$$